examples/incr_faa/FaaA.v
@@ -20,7 +20,7 @@ Module FaaA. Section FaaA.
         trigger (Guarantee ((b, ofs) ↦ Vint (v + 1)));;;
       𝒴;;; Ret tt.
 
-  Definition fnsems : gmap (option string) (option (emask * (option fspec * fbody))) :=
+  Definition fnsems : fnsemmap :=
     {[Some FaaHdr.faa2 := Some (msk_scp scopes msk_true, (None, cfunU faa2))]}.
 
   Program Definition smod : SMod.t := {|
