examples/incr_faa/IncrAll.v
@@ -1,4 +1,4 @@
-Require Import CRIS Cancel.
+Require Import CRIS Cancel SMod.
 Require Import MemI MemA MemIAproof ImpPrelude.
 Require Import SchHeader SchI SchA SchIAproof SchTactics.
 Require Import FaaHeader ClientI ClientA ClientIA FaaI FaaA FaaIA.
@@ -28,37 +28,26 @@ Module ClientAll.
   Qed.
 
   (* source module *)
-  Local Definition sp_user_s : spl_type := ClientA.sp ⊤.
-  Local Definition smod_src : SMod.t := (ClientA.smod ⊤) ☆ (SchA.smod sp_user_s).
-  Local Definition mod_top : Mod.t := SMod.to_mod sp_none (SMod.cancel smod_src).
+  Local Definition sp_user_s : specmap := ClientA.sp nroot.
+  Local Definition smod_src : SMod.t := (ClientA.smod nroot) ☆ (SchA.smod ⊤ sp_user_s).
+  Local Definition mod_top : Mod.t := SMod.to_mod ∅ (SMod.cancel smod_src).
   Local Definition mod_tgt : Mod.t := ClientI.t ★ FaaI.t ★ (MemI.t csl genv) ★ (SchI.t).
 
-  Local Definition sp : string → option fspec := sp_from smod_src.
+  Local Definition sp : specmap := SMod.conc_sp_from smod_src.
   Local Definition mod_src : Mod.t := SMod.to_mod sp smod_src.
 
-  (* Local Definition SchInSp0: sp_incl (SchAS.sp ⊤ (to_sp [])) (to_sp (SchAS.sp ⊤ (to_sp []))).
+  Local Definition SchInSp : (SchA.sp sp_user_s ⊤) ⊆ sp.
   Proof.
-    split; [|refl]. rewrite /SchAS.sp; unseal CRIS. prove_nodup.
-  Qed. *)
-  Local Definition SchInSp : sp_incl (SchA.sp sp_user_s ⊤) sp.
-  Proof.
-    rewrite /SchA.sp; unseal CRIS.
-    split; [prove_nodup|].
-    intros ??; ss; des_ifs; des_sumbool; clarify; intros INV; inv INV;
-      rewrite /sp /smod_src /sp_from /= /to_sp /=; des_ifs; ss.
+    repeat try eapply insert_subseteq_l; last apply map_empty_subseteq;
+      rewrite lookup_insert_ne // lookup_kmap_Some; eexists (Some _); split; ss.
   Qed.
-  Local Definition UserInSp : sp_incl sp_user_s sp.
+  Local Definition UserInSp : sp_user_s ⊆ sp.
   Proof.
-    rewrite /sp_user_s /ClientA.sp /MemA.sp; unseal CRIS.
-    split; [prove_nodup|].
-    intros ??; ss; des_ifs; des_sumbool; clarify; intros INV; inv INV;
-      rewrite /sp /smod_src /sp_from /= /to_sp /=; des_ifs; ss.
+    repeat try eapply insert_subseteq_l; last apply map_empty_subseteq;
+      rewrite lookup_insert_ne // lookup_kmap_Some; eexists (Some _); split; ss.
   Qed.
-  Local Definition MainInSp : spl_sub (ClientA.sp ⊤) sp_user_s.
-  Proof.
-    rewrite /spl_sub /sp_user_s /ClientA.sp /ClientA.incr_spec /=.
-    ii; rewrite ->eq_rel_dec_correct in *; des_ifs.
-  Qed.
+  Local Definition MainInSp : (ClientA.sp nroot) ⊆ sp_user_s.
+  Proof. by reflexivity. Qed.
   (* Local Definition MemInSp : sp_incl MemA.sp sp.
   Proof.
     ii; rewrite /sp /SchAS.sp /MemA.sp /ClientA.sp; unseal CRIS; split; [prove_nodup|ii].
@@ -66,31 +55,54 @@ Module ClientAll.
   Qed. *)
 
   Local Definition init_cond : iProp Σ :=
-    MemA.init_cond csl genv ∗ SchA.init_cond ∗ ClientIA.ClientIA.init_cond ⊤.
+    MemA.init_cond csl genv ∗ SchA.init_cond.
   (* Local Definition main_fsp : fspec := ClientA.main_spec ⊤ 1%Qp. *)
 
+  Lemma mod_top_wf : Mod.wf mod_top.
+  Proof.
+    rewrite /mod_top SMod.cancel_add SMod.to_mod_add. eapply Mod.add_wf.
+    { econs; eauto.
+      rewrite /ClientA.smod /= /ClientA.fnsems !fmap_insert !fmap_empty; mod_tac ss.
+    }
+    { econs; eauto.
+      { rewrite /SchA.smod /= /SchA.fnsems !fmap_insert !fmap_empty; mod_tac ss. }
+      { ss; rewrite /SchA.scopes; multiset_solver. }
+    }
+    { set_solver. }
+    { set_solver. }
+  Qed.
   (* Apply cancellation to linked spec module *)
   Lemma cancel_src :
-    refines (mod_top, init_cond ∗ TIDAUTH 0 ∗ YIELDAUTH 1)%I (mod_src, init_cond).
+    refines
+      (mod_top, init_cond ∗ TID 0 ∗ YIELD 0 ∗ winv (⊤, ⊤) ∗ emp ∗ TIDAUTH 0 ∗ YIELDAUTH 1)%I
+      (mod_src, init_cond).
   Proof.
     eapply Cancel.cancellation.
-    { ii; des; subst; inv FIND; ss.
-      rewrite !eq_rel_dec_correct in H0; des_ifs.
+    { apply SMod.cancellable_add; r; rewrite /= /ClientA.fnsems /SchA.fnsems; mod_tac ss. }
+    { apply mod_top_wf. }
+    { assert (Ht : SMod.conc_sp_from smod_src !! speckey_entry =
+        fsp_some (fspec_sch (↑nroot) fspec_trivial)); last (rewrite Ht; clear Ht).
+      { rewrite lookup_insert_ne // lookup_kmap_Some; exists None; split; ss. }
+       eexists _, _; splits.
+      { ss; exists (0, 0, tt); split; refl. }
+      { rewrite !nclose_nroot. iIntros "[$ [$ [$ ?]]]"; ss. admit. }
+      { unfold_pre_post. iIntros "% % [_ [_ $]]". }
     }
-  Qed.
+  Admitted.
 
   (* Refinement between spec/impl of whole program (linked module) *)
   Lemma src_tgt : refines (mod_src, init_cond) (mod_tgt, emp%I).
   Proof.
     eapply ctxr_refines.
-    rewrite /mod_src /mod_tgt /smod_src !add_interp_comm.
+    rewrite /mod_src /mod_tgt /smod_src.
 
     (* abstraction of Sch *)
     etrans; cycle 1.
     { do 3 ctxr_drop.
-      eapply main_adequacy, SchIA.sim.
+      eapply SchIA.ctxr.
       - apply SchInSp.
       - apply UserInSp.
+      - rewrite dom_insert elem_of_union; left; apply elem_of_singleton; ss.
     }
 
     (* abstraction of Mem *)
@@ -109,10 +121,9 @@ Module ClientAll.
     (* abstraction of Incr *)
     etrans; cycle 1.
     { ctxr_drop.
-      eapply ClientIA.ctxr.
-      - instantiate (1:=⊤). set_solver.
+      eapply ClientIA.ctxr; cycle 2.
       - apply MainInSp.
-      - apply SchInSp.
+      - rewrite nclose_nroot. apply SchInSp.
     }
 
     etrans; cycle 1.
@@ -127,13 +138,11 @@ Module ClientAll.
     rewrite /SchA.t /ClientA.t /MemA.t.
     unseal CRIS.
     ctxr_rotate.
-    
-    eapply ctxr_cond_strengthen.
-    { iIntros "[? [? ?]]". iFrame. }
+    rewrite SMod.to_mod_add /init_cond //.
   (*SLOW*)Qed.
 
   Lemma top_tgt :
-    refines (mod_top, init_cond ∗ TIDAUTH 0 ∗ YIELDAUTH 1)%I
+    refines (mod_top, init_cond ∗ TID 0 ∗ YIELD 0 ∗ winv (⊤, ⊤) ∗ emp ∗ TIDAUTH 0 ∗ YIELDAUTH 1)%I
             (mod_tgt, emp%I).
   Proof.
     etrans.
@@ -141,14 +150,37 @@ Module ClientAll.
     { eapply src_tgt. }
   Qed.
 
-  Lemma tgt_wf:
-    Mod.wf mod_tgt.
+  Lemma tgt_wf : Mod.wf mod_tgt.
   Proof.
-    rewrite /mod_tgt /ClientI.t /FaaI.t /MemI.t /SchI.t; unseal CRIS; prove_nodup.
+    rewrite /mod_tgt; eapply Mod.add_wf.
+    { econs; eauto.
+      rewrite /ClientA.smod /= /ClientA.fnsems !fmap_insert !fmap_empty; mod_tac ss.
+    }
+    { eapply Mod.add_wf.
+      { econs; eauto.
+      rewrite /ClientA.smod /= /ClientA.fnsems !fmap_insert !fmap_empty; mod_tac ss.
+      }
+      { eapply Mod.add_wf.
+        { econs; eauto.
+          { rewrite /ClientA.smod /= /ClientA.fnsems !fmap_insert !fmap_empty; mod_tac ss. }
+          { ss; rewrite /MemI.scopes; multiset_solver. }
+        }
+        { econs; eauto.
+          { rewrite /= !fmap_insert !fmap_empty; mod_tac ss. }
+          { ss; rewrite /SchI.scopes; multiset_solver. }
+        }
+        { set_solver. }
+        { set_solver. }
+      }
+      { rewrite Mod.dom_fnsems_add; set_solver. }
+      { set_solver. }
+    }
+    { rewrite !Mod.dom_fnsems_add; set_solver. }
+    { set_solver. }
   Qed.
 
   Lemma init_cond_valid:
-    ∃ rs, ✓ rs ∧ (Own rs ⊢ |==> init_cond ∗ TIDAUTH 0 ∗ YIELDAUTH 1).
+    ∃ rs, ✓ rs ∧ (Own rs ⊢ |==> init_cond ∗ TID 0 ∗ YIELD 0 ∗ winv (⊤, ⊤) ∗ emp ∗ TIDAUTH 0 ∗ YIELDAUTH 1).
   Proof.
     exists (irΣ ⋅ ir_own_admin). split.
     - apply irΣ_valid.
@@ -170,7 +202,7 @@ Module ClientAll.
     hexploit H; eauto using tgt_wf. clear H; intros [WF H].
     assert (IV:= init_cond_valid). des.
     destruct (H rs); des; et.
-    rewrite IV0 /init_cond /ClientIA.ClientIA.init_cond /ClientA.init_cond.
-    rewrite {1}winv_split_empty. iIntros ">[[$ [$ [[$ $] $]]] $]". done.
+    rewrite IV0 /init_cond.
+    rewrite {1}winv_split_empty. iIntros ">[[$ $] [$ [$ [[? ?] ?]]]]". iFrame. done.
   (*SLOW*)Qed.
 End ClientAll.
